import Relation.Binary.PropositionalEquality as Eq
open Eq using (_≡_; refl; sym; trans; cong)
open Eq.≡-Reasoning
open import Data.Bool using (Bool; true; false; T; _∧_; _∨_; not)
open import Data.Nat using (ℕ; zero; suc; _+_; _*_; _∸_; _≤_; s≤s; z≤n)
open import Data.Nat.Properties using
  (+-assoc; +-identityˡ; +-identityʳ; *-assoc; *-identityˡ; *-identityʳ; *-distribʳ-+)
open import Relation.Nullary using (¬_; Dec; yes; no)
open import Data.Product using (_×_; ∃; ∃-syntax) renaming (_,_ to ⟨_,_⟩)
open import Function using (_∘_)
open import Level using (Level)
open import plfa.part1.Isomorphism using (_≃_; _⇔_)

data List (A : Set) : Set where
  []  : List A
  _∷_ : A → List A → List A

infixr 5 _∷_

_ : List ℕ
_ = 0 ∷ 1 ∷ 2 ∷ []

data List′ : Set → Set where
  []′  : ∀ {A : Set} → List′ A
  _∷′_ : ∀ {A : Set} → A → List′ A → List′ A

_ : List ℕ
_ = _∷_ {ℕ} 0 (_∷_ {ℕ} 1 (_∷_ {ℕ} 2 ([] {ℕ})))

{-# BUILTIN LIST List #-}

pattern [_] z = z ∷ []
pattern [_,_] y z = y ∷ z ∷ []
pattern [_,_,_] x y z = x ∷ y ∷ z ∷ []
pattern [_,_,_,_] w x y z = w ∷ x ∷ y ∷ z ∷ []
pattern [_,_,_,_,_] v w x y z = v ∷ w ∷ x ∷ y ∷ z ∷ []
pattern [_,_,_,_,_,_] u v w x y z = u ∷ v ∷ w ∷ x ∷ y ∷ z ∷ []

infixr 5 _++_

_++_ : ∀ {A : Set} → List A → List A → List A
[]       ++ ys  =  ys
(x ∷ xs) ++ ys  =  x ∷ (xs ++ ys)


_ : [ 0 , 1 , 2 ] ++ [ 3 , 4 ] ≡ [ 0 , 1 , 2 , 3 , 4 ]
_ = refl

++-assoc : ∀ {A : Set} (xs ys zs : List A)
  → (xs ++ ys) ++ zs ≡ xs ++ (ys ++ zs)
++-assoc [] ys zs = refl
++-assoc (x ∷ xs) ys zs = 
  begin
    (x ∷ xs ++ ys) ++ zs
  ≡⟨⟩
    x ∷ (xs ++ ys) ++ zs
  ≡⟨⟩
    x ∷ ((xs ++ ys) ++ zs)
  ≡⟨ cong (x ∷_) (++-assoc xs ys zs) ⟩
    x ∷ (xs ++ (ys ++ zs))
  ≡⟨⟩
    x ∷ xs ++ (ys ++ zs)
  ∎

++-identityˡ : ∀ {A : Set} (xs : List A) → [] ++ xs ≡ xs
++-identityˡ xs = refl

++-identityʳ : ∀ {A : Set} (xs : List A) → xs ++ [] ≡ xs
++-identityʳ [] = refl
++-identityʳ (x ∷ xs) =
  begin
    (x ∷ xs) ++ []
  ≡⟨⟩
    x ∷ (xs ++ [])
  ≡⟨ cong (x ∷_) (++-identityʳ xs) ⟩
    x ∷ xs
  ∎

length : ∀ {A : Set} → List A → ℕ
length []        =  zero
length (x ∷ xs)  =  suc (length xs)

_ : length [ 0 , 1 , 2 ] ≡ 3
_ = refl

length-++ : ∀ {A : Set} (xs ys : List A)
  → length (xs ++ ys) ≡ length xs + length ys
length-++ {A} [] ys =
  begin
    length ([] ++ ys)
  ≡⟨⟩
    length ys
  ≡⟨⟩
    length {A} [] + length ys
  ∎
length-++ (x ∷ xs) ys =
  begin
    length ((x ∷ xs) ++ ys)
  ≡⟨⟩
    suc (length (xs ++ ys))
  ≡⟨ cong suc (length-++ xs ys) ⟩
    suc (length xs + length ys)
  ≡⟨⟩
    length (x ∷ xs) + length ys
  ∎

reverse : ∀ {A : Set} → List A → List A
reverse []        =  []
reverse (x ∷ xs)  =  reverse xs ++ [ x ]

_ : reverse [ 0 , 1 , 2 ] ≡ [ 2 , 1 , 0 ]
_ = refl

shunt : ∀ {A : Set} → List A → List A → List A
shunt []       ys  =  ys
shunt (x ∷ xs) ys  =  shunt xs (x ∷ ys)


shunt-reverse : ∀ {A : Set} (xs ys : List A)
  → shunt xs ys ≡ reverse xs ++ ys
shunt-reverse [] ys = refl
shunt-reverse (x ∷ xs) ys =
  begin
    shunt (x ∷ xs) ys
  ≡⟨⟩
    shunt xs (x ∷ ys)
  ≡⟨ shunt-reverse xs (x ∷ ys) ⟩
    reverse xs ++ (x ∷ ys)
  ≡⟨⟩
    reverse xs ++ ([ x ] ++ ys)
  ≡⟨ sym (++-assoc (reverse xs) [ x ] ys) ⟩
    (reverse xs ++ [ x ]) ++ ys
  ≡⟨⟩
    reverse (x ∷ xs) ++ ys
  ∎

reverse′ : ∀ {A : Set} → List A → List A
reverse′ xs = shunt xs []

reverses : ∀ {A : Set} (xs : List A)
  → reverse′ xs ≡ reverse xs
reverses xs =
  begin
    reverse′ xs
  ≡⟨⟩
    shunt xs []
  ≡⟨ shunt-reverse xs [] ⟩
    reverse xs ++ []
  ≡⟨ ++-identityʳ (reverse xs) ⟩
    reverse xs
  ∎

map : ∀ {A B : Set} → (A → B) → List A → List B
map f []        =  []
map f (x ∷ xs)  =  f x ∷ map f xs

_ : map suc [ 0 , 1 , 2 ] ≡ [ 1 , 2 , 3 ]
_ = refl


